src/hls/RTLBlockgen.v
@@ -16,7 +16,6 @@
  * along with this program.  If not, see <https://www.gnu.org/licenses/>.
  *)
 
-(* [[file:../../docs/basic-block-generation.org::rtlblockgen-imports][rtlblockgen-imports]] *)
 Require compcert.backend.RTL.
 Require Import compcert.common.AST.
 Require Import compcert.lib.Maps.
@@ -28,7 +27,6 @@ Require Import vericert.hls.RTLBlockInstr.
 Require Import vericert.hls.RTLBlock.
 
 #[local] Open Scope positive.
-(* rtlblockgen-imports ends here *)
 
 Lemma comparison_eq: forall (x y : comparison), {x = y} + {x <> y}.
 Proof.
@@ -148,15 +146,19 @@ Defined.
 Definition ceq {A: Type} (eqd: forall a b: A, {a = b} + {a <> b}) (a b: A): bool :=
   if eqd a b then true else false.
 
-(* [[file:../../docs/basic-block-generation.org::rtlblockgen-main][rtlblockgen-main]] *)
 Parameter partition : RTL.function -> Errors.res function.
 
-(** [find_block max nodes index]: Does not need to be sorted, because we use filter and the max fold
-    function to find the desired element. *)
+(*|
+``find_block max nodes index``: Does not need to be sorted, because we use
+filter and the max fold function to find the desired element.
+
+    .. coq::
+|*)
+
 Definition find_block (max: positive) (nodes: list positive) (index: positive) : positive :=
   List.fold_right Pos.min max (List.filter (fun x => (index <=? x)) nodes).
 
-(*Compute find_block (2::94::28::40::19::nil) 40.*)
+(*Compute find_block 100 (2::94::48::39::19::nil) 40.*)
 
 Definition check_instr (n: positive) (istr: RTL.instruction) (istr': instr) :=
   match istr, istr' with
@@ -287,4 +289,3 @@ Definition transl_fundef := transf_partial_fundef transl_function.
 
 Definition transl_program : RTL.program -> Errors.res program :=
   transform_partial_program transl_fundef.
-(* rtlblockgen-main ends here *)
